\documentclass[12pt]{article}

\usepackage{hyperref}
\usepackage{amsmath, amssymb, amsthm}
\usepackage[sort&compress,numbers]{natbib}
\usepackage{doi}
\usepackage[margin=0.8in]{geometry}
%\textheight23cm \topmargin-20mm  
%\textwidth175mm  
%\oddsidemargin=0mm
%\evensidemargin=0mm
%

\usepackage{amsmath, amssymb, amsthm, mathtools}

\newtheorem{lemma}{Lemma}
\newtheorem{prop}{Proposition}
\newtheorem{theorem}{Theorem}
\newtheorem{coro}{Corollary}


\theoremstyle{definition}
\newtheorem{defi}{Definition}


\theoremstyle{remark}
\newtheorem{remark}{Remark}

\def\Me{\mathcal M}
\def\Ee{\mathcal E}
\def\Fe{\mathcal F}
\def\Ra{\mathcal R}
\def\Ne{\mathcal N}
\def \Tr{\mathrm{Tr}\,}
\def\Se {\mathcal S}
\def\ffi{\varphi}
\def\supp{\mathrm{supp}}
\def\<{\langle\.}
\def\>{\.\rangle}

\title{Equality in DPI for sandwiched R\'enyi divergence}
\author{Anna Jen\v cov\'a}

\begin{document}

\maketitle

Below, $\gamma:\Ne\to \Me$ is a normal positive unital map, $\psi,\ffi\in \Me_*^+$ and we
put $\psi_0=\psi\circ\gamma$, $\ffi_0=\ffi\circ\gamma$. We consider the following equality
\begin{equation}\label{eq:dpi_equality}
D_{\alpha,z}(\psi\|\ffi)=D_{\alpha,z}(\psi_0\|\ffi_0)
\end{equation}
where $\alpha>1$ and $\max\{\alpha/2,\alpha-1\}\le z\le \alpha$. We put $q=\frac
z{\alpha-1}$. In the case $\alpha=z$ we have $D_{\alpha,\alpha}=\tilde D_\alpha$ is the
sandwiched R\'enyi divergence. We assume $D_{\alpha,z}(\psi\|\ffi)<\infty$, then by DPI we
also have $D_{\alpha,z}(\psi_0\|\ffi_0)<\infty$. Hence there are  $y\in L_{2z}(\Me)$ and
$y_0\in L_{2z}(\Ne)$ such that 
\[
h_\psi^{\alpha\over 2z}=yh_\ffi^{\alpha-1\over
2z},\qquad h_{\psi_0}^{\alpha\over 2z}=y_0h_{\ffi_0}^{\alpha-1\over
2z}.
\]

\begin{lemma}\cite[Lemma 3.10]{hiai2024ontheproperties}\label{lemma:le} Let $\gamma:\Ne\to\Me$ be a normal positive unital map.
Let $\gamma^*_{\ffi,q}:L_q(\Ne)\to L_q(\Me)$ be the contraction as in \cite[Lemma 3.1]{hiai2024ontheproperties}.
Let $\bar w:(y^*y)^{\alpha-1}\in L_q(\Me)$ and $\bar w_0:=(y_0^*y_0)^{\alpha-1}\in
L_q(\Ne)$. Then \eqref{eq:dpi_equality} holds if and only if
\begin{equation}\label{eq:dpiw}
\bar w=\gamma^*_{\ffi,q}(\bar w_0)\quad \text{and}\quad
\Tr \bigl(\bar w_0^q\bigr)=\Tr \bigl(\gamma^*_{\varphi,q}(\bar w_0)^q\bigr).
\end{equation}


\end{lemma}

We show that \eqref{eq:dpi_equality} implies reversibility of $\gamma$ for the sandwiched
R\'enyi divergence. 

\begin{theorem}\label{thm:sandwiched} Let $\gamma:\Ne\to \Me$ be a normal positive unital
map. Let $\psi,\ffi\in \Me_*^+$ be such that  $\tilde
D_\alpha(\psi\|\ffi)<\infty$ for some $\alpha>1$. Then $\tilde D_\alpha(\psi\|\ffi)=\tilde
D_\alpha(\psi_0\|\ffi_0)$ if and only if $\psi\circ\gamma\circ\gamma^*_\ffi=\psi$.


\end{theorem}

\begin{proof} Let $\bar w$ and $\bar w_0$ be as in Lemma \ref{lemma:le}. Let $\omega\in
\Me_*^+$ and $\omega_0\in \Ne_*^+$ be such that
\[
h_\omega=h_\ffi^{\frac1{2\alpha}}\bar wh_\ffi^{\frac1{2\alpha}},\qquad
h_{\omega_0}=h_{\ffi_0}^{\frac1{2\alpha}}\bar w_0h_{\ffi_0}^{\frac1{2\alpha}}.
\]
Note that in this
case $q=\tfrac{\alpha}{\alpha-1}$. Then $h_\omega\in L_q(\Me,\ffi)$ and $h_{\omega_0}\in
L_q(\Ne,\ffi_0)$. Assume the equality in DPI holds, then by Lemma
\ref{lemma:le} we have
\[
\|h_\omega\|_{q,\ffi}=\|\bar w\|_q=\|\gamma^*_{\ffi,q}(\bar
w_0)\|_q=\|\bar w_0\|_q=\|h_{\omega_0}\|_{q,\ffi_0}=:l
\]
and using also \cite[Lemma 3.1]{hiai2024ontheproperties}, we have
\[
(\gamma^*_\ffi)_*(h_{\omega_0})=h_\ffi^{\frac1{2\alpha}}\gamma^*_{\ffi,q}(\bar
w_0)h_\ffi^{\frac1{2\alpha}}=h_\omega.
\]
Let $f_{h_{\omega_0},q}$ and $f_{h_\omega,q}$ be the functions as in \cite[Eq.
(9)]{jencova2018renyi}, so that
\[
f_{h_{\omega_0},q}(s)=l^{1-sq}h_{\ffi_0}^{1-s\over 2}\bar w_0^{qs}h_{\ffi_0}^{1-s\over 2},
\qquad f_{h_\omega,q}(s)=l^{1-sq}h_{\ffi}^{1-s\over 2}\bar w^{qs}h_{\ffi}^{1-s\over 2}, \qquad s\in
S,
\]
here $S$ is the strip $S=\{s\in \mathbb C,\ 0\le \mathrm{Re}(s)\le 1\}$. Note that we have
$f_{h_\omega,q}(1/q)=h_\omega$ and 
\[
\sup_t\|f_{h_{\omega_0},q}(it)\|_{\infty,\ffi_0}=
\sup_t\|f_{h_{\omega_0},q}(1+it)\|_{1}=l=\|h_{\omega_0}\|_{q,\ffi},
\]
similarly for $f_{h_{\omega},q}$. 


Put $g(s):=(\gamma^*_\ffi)_*(f_{h_{\omega_0},q}(s))$, $s\in S$, then $g$ is a bounded continuous
function $S\to L_1(\Me)$, analytic in the interior and such  such that $g(1/q)=h_\omega$.
Since $(\gamma^*_\ffi)_*$ is a contraction 
$L_r(\Ne,\ffi_0)\to L_r(\Me,\ffi)$ for any $1\le r\le \infty$, we have by the Hadamard
three lines theorem (see e.g. \cite[Thm. 2.10]{jencova2018renyi} in this context) 
\begin{align*}
\|g(1/q)\|_{q,\ffi}&\le
\bigl(\sup_t\|g(it)\|_{\infty,\ffi}\bigr)^{1-1/q}\bigl(\sup_t\|g(1+it)\|_{1}\bigr)^{1/q}\\
&\le
\bigl(\sup_t\|f_{h_{\omega_0},q}(it)\|_{\infty,\ffi}\bigr)^{1-1/q}\bigl(\sup_t\|f_{h_{\omega_0},q}(1+it)\|_{1}\bigr)^{1/q}
=\|h_{\omega_0}\|_{q,\ffi_0}=\|g(1/q)\|_{q,\ffi}.
\end{align*}
It follows that $g$ satisfies equality in the Hadamard three lines theorem and we must
have
\[
\sup_t\|g(it)\|_{\infty,\ffi}=\sup_t\|f_{h_{\omega_0},q}(it)\|_{\infty,\ffi_0}=
\sup_t\|f_{h_{\omega_0},q}(1+it)\|_{1}=\sup_t\|g(1+it)\|_{1}.
\]
By \cite[Thm. 2.10]{jencova2018renyi}, this  implies that $g(s)=f_{h_\omega,q}(s)$
for all $s\in S$. For $s=1/\alpha$ this implies
\[
h_\psi=h_\ffi^{q-1\over 2q}y^*yh_\ffi^{q-1\over 2q}=(\gamma^*_\ffi)_*(h_{\ffi_0}^{q-1\over
2q}y_0^*y_0h_{\ffi_0}^{q-1\over 2q})=(\gamma^*_\ffi)_*(h_{\psi_0}),
\]
that is, $\psi\circ\gamma\circ\gamma^*_\ffi=\psi$. The converse is clear from DPI.

\end{proof}

For $\alpha\ne z$, we still need 2-positivity of $\gamma$ for the proof that
\eqref{eq:dpi_equality} implies sufficiency. Using Theorem \ref{thm:sandwiched} and
similar arguments as in its proof, we can prove equivalent conditions for
\eqref{eq:dpi_equality} of the form 
\[
\gamma_*((y^*y)^z)=(y_0^*y_0)^z
\]
for $\alpha>1$ and
\[
\gamma^*((h_\psi^{\alpha\over 2z}h_\ffi^{1-\alpha\over z}h_\psi^{\alpha\over
2z})^z)=(h_{\psi_0}^{\alpha\over 2z}h_{\ffi_0}^{1-\alpha\over z}h_{\psi_0}^{\alpha\over 2z})^z
\]
for $\alpha\in (0,1)$, $z>\alpha$,
\[
\gamma^*((h_\ffi^{1-\alpha\over 2z}h_\psi^{\alpha\over z}h_\ffi^{1-\alpha\over
2z})^z)=(h_{\ffi_0}^{1-\alpha\over 2z}h_{\psi_0}^{\alpha\over z}h_{\ffi_0}^{1-\alpha\over 2z})^z
\]
for $\alpha\in (0,1)$, $z>1-\alpha$ (all within the DPI bounds).
This is related but not quite the same as the conditions by Zhang
\cite{zhang2020equality}. For example, if $\psi\sim\ffi$ the equality in the last case
becomes
\[
\gamma_*((h_\ffi^{1-\alpha\over2z}\bar
a^{-1}h_\ffi^{1-\alpha\over2z})^{z\over 1-\alpha}=(h_{\ffi_0}^{1-\alpha\over2z}\bar
a_0^{-1}h_{\ffi_0}^{1-\alpha\over2z})^{z\over 1-\alpha},
\]
whereas the corresponding Zhang's condition is
\[
\gamma_*((\bar a^{-\frac12}h_\ffi^{1-\alpha\over z}\bar a^{-\frac12})^{z\over 1-\alpha})=
(\bar a_0^{-\frac12}h_{\ffi_0}^{1-\alpha\over z}\bar a_0^{-\frac12})^{z\over 1-\alpha}.
\]

%\bibliography{alphaz}
%\bibliographystyle{abbrvnat}

\begin{thebibliography}{2}
\providecommand{\natexlab}[1]{#1}
\providecommand{\url}[1]{\texttt{#1}}
\expandafter\ifx\csname urlstyle\endcsname\relax
  \providecommand{\doi}[1]{doi: #1}\else
  \providecommand{\doi}{doi: \begingroup \urlstyle{rm}\Url}\fi

\bibitem{hiai2024ontheproperties} 
F.~Hiai, A.~Jen\v cov\'a. On the properties of $\alpha-z$-R\'enyi divergences on von
Neumann algebras. In preparation.

\bibitem[Jen{\v c}ov{\'a}(2018)]{jencova2018renyi}
A.~Jen{\v c}ov{\'a}.
\newblock {R{\'e}nyi relative entropies and noncommutative $L_p$-spaces}.
\newblock \emph{Annales Henri Poincar{\'e}}, 19:\penalty0 2513--2542, 2018.
\newblock \doi{10.1007/s00023-018-0683-5}.

\bibitem[Zhang(2020)]{zhang2020equality}
H.~Zhang.
\newblock Equality conditions of data processing inequality for $\alpha$-z
  R{\'e}nyi relative entropies.
\newblock \emph{Journal of Mathematical Physics}, 61\penalty0 (10), 2020.
\newblock \doi{10.1063/5.0022787}.

\end{thebibliography}



\end{document}


